src/lib/inst/Kuiper.MatMul.U64.fst
@@ -5,7 +5,7 @@ open Kuiper
 open Kuiper.MatMul
 
 [@@CPrologue "__global__"]
-let kernel_u64 = kernel #u64 R.c_row_major R.c_row_major R.c_row_major
+let kernel_u64 = kernel #u64 R.row_major R.row_major R.row_major
 
-let matmul_u64 : matmul_ty u64 R.c_row_major R.c_row_major R.c_row_major =
+let matmul_u64 : matmul_ty u64 R.row_major R.row_major R.row_major =
   matmul kernel_u64
