src/lib/inst/Kuiper.MatMul.U64.fsti
@@ -5,4 +5,4 @@ open Kuiper
 open Kuiper.MatMul
 module R = Kuiper.Matrix.Reprs
 
-val matmul_u64 : matmul_ty u64 R.c_row_major R.c_row_major R.c_row_major
+val matmul_u64 : matmul_ty u64 R.row_major R.row_major R.row_major
